rt abstract: size parametrise SchedContext

spec/abstract/Structures_A.thy
@@ -446,7 +446,13 @@ record sched_context =
   sc_replies    :: "obj_ref list"
 
 definition "MIN_REFILLS = 2"
-(* what is the difference between MIN_REFILLS (=2) and seL4_MinRefills (=0) ? *)
+definition "MIN_BUDGET = 2 * kernelWCET_ticks"
+definition "MIN_BUDGET_US = 2 * kernelWCET_us"
+
+definition "min_sched_context_bits = 8"
+definition "core_sched_context_bytes = (8 * 32 + (5 * 8))" (* RT *)
+definition "refill_size_bytes = 2 * 8"
+definition "max_extra_refills sz = ((1 << sz) - core_sched_context_bytes) / refill_size_bytes"
 
 definition
   default_sched_context :: sched_context where
@@ -464,12 +470,10 @@ definition
 
 record reply =
   reply_tcb :: "obj_ref option"
-(*  reply_caller :: "obj_ref option"
-  reply_callee :: "obj_ref option"*)
   reply_sc     :: "obj_ref option"
 
 definition
-  "default_reply = \<lparr> reply_tcb = None, (*reply_caller = None, reply_callee = None,*) reply_sc = None \<rparr>"
+  "default_reply = \<lparr> reply_tcb = None,  reply_sc = None \<rparr>"
 
 text {*
 All kernel objects are CNodes, TCBs, Endpoints, Notifications or architecture
@@ -480,7 +484,7 @@ datatype kernel_object
          | TCB tcb
          | Endpoint endpoint
          | Notification notification
-         | SchedContext sched_context
+         | SchedContext sched_context nat
          | Reply reply
          | ArchObj (the_arch_obj: arch_kernel_obj)
 
@@ -501,6 +505,12 @@ definition
   well_formed_cnode_n :: "nat \<Rightarrow> cnode_contents \<Rightarrow> bool" where
  "well_formed_cnode_n n \<equiv> \<lambda>cs. dom cs = {x. length x = n}"
 
+text {* checks for the scheduling context size *}
+
+definition valid_sched_context_size :: "nat \<Rightarrow> bool" where
+  "valid_sched_context_size n \<equiv> min_sched_context_bits \<le> n \<and> n \<le> untyped_max_bits"
+
+
 primrec
   obj_bits :: "kernel_object \<Rightarrow> nat"
 where
@@ -508,7 +518,7 @@ where
 | "obj_bits (TCB t) = tcb_bits"
 | "obj_bits (Endpoint ep) = endpoint_bits"
 | "obj_bits (Notification ntfn) = ntfn_bits" (* RT ARM: 5*)
-| "obj_bits (SchedContext sc) = 8"
+| "obj_bits (SchedContext sc n) = n"  (* n \<ge> 8 *)
 | "obj_bits (Reply r) = 4"
 | "obj_bits (ArchObj ao) = arch_kobj_size ao"
 
@@ -739,5 +749,74 @@ proof -
   qed
   thus ?thesis unfolding msg_align_bits_def max_ipc_length_def by simp
 qed
+
+
+section "simple kernel objects"
+(* to be used for abstraction unifying kernel objects other than TCB, CNode, and SchedContext *)
+
+context begin interpretation Arch .
+
+requalify_types
+  aa_type
+requalify_consts
+  aa_type
+
+end
+
+text {* An alternative formulation that allows abstraction over type: *}
+
+datatype a_type =
+    ATCB
+  | AEndpoint
+  | ANTFN
+  | ASchedContext nat
+  | AReply
+  | ACapTable nat
+  | AGarbage nat -- "number of bytes of garbage"
+  | AArch aa_type
+
+definition
+  a_type :: "kernel_object \<Rightarrow> a_type"
+where
+ "a_type ob \<equiv> case ob of
+           CNode sz cspace           \<Rightarrow> if well_formed_cnode_n sz cspace
+                                        then ACapTable sz else AGarbage (cte_level_bits + sz)
+         | TCB tcb                   \<Rightarrow> ATCB
+         | Endpoint endpoint         \<Rightarrow> AEndpoint
+         | SchedContext sc n         \<Rightarrow> if valid_sched_context_size n
+                                        then ASchedContext n else AGarbage n
+         | Reply r                   \<Rightarrow> AReply
+         | Notification notification \<Rightarrow> ANTFN
+         | ArchObj ao                \<Rightarrow> AArch (aa_type ao)"
+
+(***)
+
+definition
+  partial_inv :: "('a \<Rightarrow> 'b) \<Rightarrow> ('b \<Rightarrow> 'a option)"
+where
+  "partial_inv f x = (if \<exists>!y. f y = x then Some (THE y. f y = x) else None)"
+
+lemma proj_inj: "inj f \<Longrightarrow> (partial_inv f ko = Some v) = (f v = ko)"
+  by (auto simp: partial_inv_def the_equality injD)
+
+lemma inj_Endpoint: "inj Endpoint" by (auto intro: injI)
+lemma inj_Notification: "inj Notification"  by (auto intro: injI)
+
+lemmas proj_inj_ep[simp] = proj_inj[OF inj_Endpoint]
+lemma proj_ko_type_ep[simp]: "(\<exists>v. partial_inv Endpoint  ko = Some (v::endpoint)) = (a_type ko = AEndpoint)"
+  by (cases ko; auto simp: partial_inv_def a_type_def)
+
+lemmas proj_inj_ntfn[simp] = proj_inj[OF inj_Notification]
+lemma proj_ko_type_ntfn[simp]:
+  "(\<exists>v. partial_inv Notification  ko = Some (v::notification)) = (a_type ko = ANTFN)"
+  by (cases ko; auto simp: partial_inv_def a_type_def)
+
+lemma proj_inj_reply[simp]: "(partial_inv Reply ko = Some v) = (Reply v = ko)"
+  by (auto simp: partial_inv_def)
+lemma proj_ko_type_reply[simp]: "(\<exists>v. partial_inv Reply  ko = Some (v::reply)) = (a_type ko = AReply)"
+  by (cases ko; auto simp: partial_inv_def a_type_def)
+
+abbreviation
+  "is_simple_type \<equiv> (\<lambda>ob. a_type ob \<in> {AEndpoint, ANTFN, AReply})"
 
 end
